compcomp/CminorgenproofSIM.v
@@ -19,6 +19,7 @@ Require Import CminorgenproofRestructured.
 
 Require Import sepcomp.mem_lemmas.
 Require Import sepcomp.core_semantics.
+Require Import sepcomp.core_semantics_lemmas.
 
 Require Import Coq.Program.Equality.
 
