compcomp/SelectionproofEFF.v
@@ -25,6 +25,7 @@ Require Import SelectLongproof.
 
 Require Import sepcomp.mem_lemmas.
 Require Import sepcomp.core_semantics.
+Require Import sepcomp.core_semantics_lemmas.
 Require Import sepcomp.effect_semantics.
 Require Import StructuredInjections.
 Require Import sepcomp.reach.
