compcomp/StackingproofEFF.v
@@ -41,6 +41,7 @@ Require Import Mach_eff.
 
 Require Import sepcomp.mem_lemmas.
 Require Import sepcomp.core_semantics.
+Require Import sepcomp.core_semantics_lemmas.
 Require Import sepcomp.effect_semantics.
 Require Import StructuredInjections.
 Require Import reach.
