sepcomp/closed_safety.v
@@ -1,6 +1,7 @@
 Require Import sepcomp.compcert. Import CompcertLibraries.
 
 Require Import sepcomp.core_semantics.
+Require Import sepcomp.core_semantics_lemmas.
 
 Set Implicit Arguments.
 Unset Strict Implicit.
