sepcomp/core_semantics_lemmas.v
@@ -1,0 +1,167 @@
+(*CompCert imports*)
+Require Import Events.
+Require Import Memory.
+Require Import Coqlib.
+Require Import compcert.common.Values.
+Require Import Maps.
+Require Import Integers.
+Require Import AST. 
+Require Import Globalenvs.
+Require Import msl.Axioms.
+
+Require Import sepcomp.mem_lemmas.
+Require Import sepcomp.core_semantics.
+
+Definition corestep_fun {G C M : Type} (sem : CoreSemantics G C M) :=
+  forall (m m' m'' : M) ge c c' c'',
+  corestep sem ge c m c' m' -> 
+  corestep sem ge c m c'' m'' -> 
+  c'=c'' /\ m'=m''.
+
+(**  Multistepping *)
+
+Section corestepN.
+  Context {G C M E:Type} (Sem:CoreSemantics G C M) (ge:G).
+
+  Fixpoint corestepN (n:nat) : C -> M -> C -> M -> Prop :=
+    match n with
+      | O => fun c m c' m' => (c,m) = (c',m')
+      | S k => fun c1 m1 c3 m3 => exists c2, exists m2,
+        corestep Sem ge c1 m1 c2 m2 /\
+        corestepN k c2 m2 c3 m3
+    end.
+
+  Lemma corestepN_add : forall n m c1 m1 c3 m3,
+    corestepN (n+m) c1 m1 c3 m3 <->
+    exists c2, exists m2,
+      corestepN n c1 m1 c2 m2 /\
+      corestepN m c2 m2 c3 m3.
+  Proof.
+    induction n; simpl; intuition.
+    firstorder. firstorder.
+    inv H. auto.
+    decompose [ex and] H. clear H.
+    destruct (IHn m x x0 c3 m3).
+    apply H in H2. 
+    decompose [ex and] H2. clear H2.
+    repeat econstructor; eauto.
+    decompose [ex and] H. clear H.
+    exists x1. exists x2; split; auto.
+    destruct (IHn m x1 x2 c3 m3). 
+    eauto.
+  Qed.
+
+  Definition corestep_plus c m c' m' :=
+    exists n, corestepN (S n) c m c' m'.
+
+  Definition corestep_star c m c' m' :=
+    exists n, corestepN n c m c' m'.
+
+  Lemma corestep_plus_star : forall c1 c2 m1 m2,
+    corestep_plus c1 m1 c2 m2 -> corestep_star c1 m1 c2 m2.
+  Proof. intros. destruct H as [n1 H1]. eexists. apply H1. Qed.
+
+  Lemma corestep_plus_trans : forall c1 c2 c3 m1 m2 m3,
+    corestep_plus c1 m1 c2 m2 -> corestep_plus c2 m2 c3 m3 -> 
+    corestep_plus c1 m1 c3 m3.
+  Proof. intros. destruct H as [n1 H1]. destruct H0 as [n2 H2].
+    destruct (corestepN_add (S n1) (S n2) c1 m1 c3 m3) as [_ H].
+    eexists. apply H. exists c2. exists m2. split; assumption.
+  Qed.
+
+  Lemma corestep_star_plus_trans : forall c1 c2 c3 m1 m2 m3,
+    corestep_star c1 m1 c2 m2 -> corestep_plus c2 m2 c3 m3 -> 
+    corestep_plus c1 m1 c3 m3.
+  Proof. intros. destruct H as [n1 H1]. destruct H0 as [n2 H2].
+    destruct (corestepN_add n1 (S n2) c1 m1 c3 m3) as [_ H]. 
+    rewrite <- plus_n_Sm in H.
+    eexists. apply H.  exists c2. exists m2.  split; assumption.
+  Qed.
+
+  Lemma corestep_plus_star_trans: forall c1 c2 c3 m1 m2 m3,
+    corestep_plus c1 m1 c2 m2 -> corestep_star c2 m2 c3 m3 -> 
+    corestep_plus c1 m1 c3 m3.
+  Proof. intros. destruct H as [n1 H1]. destruct H0 as [n2 H2].
+    destruct (corestepN_add (S n1) n2 c1 m1 c3 m3) as [_ H]. 
+    rewrite plus_Sn_m in H.
+    eexists. apply H.  exists c2. exists m2.  split; assumption.
+  Qed.
+
+  Lemma corestep_star_trans: forall c1 c2 c3 m1 m2 m3, 
+    corestep_star c1 m1 c2 m2 -> corestep_star c2 m2 c3 m3 -> 
+    corestep_star c1 m1 c3 m3.
+  Proof. intros. destruct H as [n1 H1]. destruct H0 as [n2 H2].
+    destruct (corestepN_add n1 n2 c1 m1 c3 m3) as [_ H]. 
+    eexists. apply H.  exists c2. exists m2.  split; assumption.
+  Qed.
+
+  Lemma corestep_plus_one: forall c m c' m',
+    corestep  Sem ge c m c' m' -> corestep_plus c m c' m'.
+  Proof. intros. unfold corestep_plus, corestepN. simpl.
+    exists O. exists c'. exists m'. eauto. 
+  Qed.
+
+  Lemma corestep_plus_two: forall c m c' m' c'' m'',
+    corestep  Sem ge c m c' m' -> corestep  Sem ge c' m' c'' m'' -> 
+    corestep_plus c m c'' m''.
+  Proof. intros. 
+    exists (S O). exists c'. exists m'. split; trivial. 
+    exists c''. exists m''. split; trivial. reflexivity.
+  Qed.
+
+  Lemma corestep_star_zero: forall c m, corestep_star  c m c m.
+  Proof. intros. exists O. reflexivity. Qed.
+
+  Lemma corestep_star_one: forall c m c' m',
+    corestep  Sem ge c m c' m' -> corestep_star c m c' m'.
+  Proof. intros. 
+    exists (S O). exists c'. exists m'. split; trivial. reflexivity. 
+  Qed.
+
+  Lemma corestep_plus_split: forall c m c' m',
+    corestep_plus c m c' m' ->
+    exists c'', exists m'', corestep  Sem ge c m c'' m'' /\ 
+      corestep_star c'' m'' c' m'.
+  Proof. intros.
+    destruct H as [n [c2 [m2 [Hstep Hstar]]]]. simpl in*. 
+    exists c2. exists m2. split. assumption. exists n. assumption.  
+  Qed.
+
+End corestepN.
+
+Section CoopCoreSemLemmas.
+Context {G C: Type}.
+Variable coopsem: CoopCoreSem G C.
+
+Lemma corestepN_fwd: forall ge c m c' m' n,
+  corestepN coopsem ge n c m c' m' -> 
+  mem_forward m m'.
+Proof.
+intros until n; revert c m.
+induction n; simpl; auto.
+inversion 1; apply mem_forward_refl; auto.
+intros c m [c2 [m2 [? ?]]].
+apply mem_forward_trans with (m2 := m2).
+apply corestep_fwd in H; auto.
+eapply IHn; eauto.
+Qed.
+
+Lemma corestep_star_fwd: forall g c m c' m'
+  (CS:corestep_star coopsem g c m c' m'), 
+  mem_forward m m'.
+Proof. 
+  intros. destruct CS. 
+  eapply corestepN_fwd. 
+  apply H.
+Qed.
+
+Lemma corestep_plus_fwd: forall g c m c' m'
+  (CS:corestep_plus coopsem g c m c' m'), 
+  mem_forward m m'.
+Proof.
+   intros. destruct CS.
+   eapply corestepN_fwd.
+   apply H.
+Qed.
+
+End CoopCoreSemLemmas.
