sepcomp/effect_semantics.v
@@ -10,6 +10,7 @@ Require Import Globalenvs.
 Require Import msl.Axioms.
 Require Import sepcomp.mem_lemmas. (*needed for definition of mem_forward etc*)
 Require Import sepcomp.core_semantics.
+Require Import sepcomp.core_semantics_lemmas.
 Require Import sepcomp.StructuredInjections.
 
  
