sepcomp/effect_simulations.v
@@ -14,6 +14,7 @@ Require Import compcert.lib.Axioms.
 
 Require Import sepcomp.mem_lemmas. (*needed for definition of mem_forward etc*)
 Require Import sepcomp.core_semantics.
+Require Import sepcomp.core_semantics_lemmas.
 Require Import sepcomp.effect_semantics.
 Require Import sepcomp.StructuredInjections.
 Require Import sepcomp.reach.
