sepcomp/forward_simulations_trans.v
@@ -23,6 +23,7 @@ Require Import sepcomp.Coqlib2.
 
 Require Import sepcomp.mem_lemmas.
 Require Import sepcomp.core_semantics.
+Require Import sepcomp.core_semantics_lemmas.
 Require Import sepcomp.forward_simulations.
 
 Require Import Wellfounded.
