sepcomp/step_lemmas.v
@@ -3,6 +3,7 @@ Require Import Coqlib.
 
 Require Import sepcomp.extspec.
 Require Import sepcomp.core_semantics.
+Require Import sepcomp.core_semantics_lemmas.
 Require Import sepcomp.forward_simulations.
 
 Section safety.
