Makefile
@@ -71,7 +71,8 @@ SEPCOMP_FILES= \
   mem_lemmas.v mem_interpolants.v mem_interpolation_defs.v \
   mem_interpolation_EE.v mem_interpolation_EI.v mem_interpolation_IE.v mem_interpolation_II.v \
   mem_interpolation_proofs.v compiler_correctness.v \
-  core_semantics.v forward_simulations.v forward_simulations_trans.v \
+  core_semantics.v core_semantics_lemmas.v \
+  forward_simulations.v forward_simulations_trans.v \
   forward_simulations_lemmas.v \
   compiler_correctness_trans.v compiler_correctness_progless_trans.v \
   safety_preservation.v \
